new queue

examples/steel/TwoLockQueue.fst
@@ -9,7 +9,9 @@ module L = FStar.List.Tot
 module U = Steel.Utils
 module Q = Queue
 
+[@@__reduce__]
 let full = full_perm
+[@@__reduce__]
 let half = half_perm full
 let fst x = fst x
 let snd x = snd x
@@ -32,14 +34,24 @@ let queue_invariant (#a:_) (head tail:q_ptr a) =
     ghost_pts_to tail.ghost half (hide (snd (reveal ht))) `star`
     Q.queue (hide (fst (reveal ht))) (hide (snd (reveal ht))))
 
-let pack_queue_invariant (#a:_) (#u:_) (head tail:q_ptr a)
+let pack_queue_invariant (#a:_) (#u:_) (x:erased (Q.t a)) (y:erased (Q.t a)) (head tail:q_ptr a)
  : SteelAtomicT unit u unobservable
-   (h_exists (fun (ht: erased (Q.t a & Q.t a)) ->
-     ghost_pts_to head.ghost half (hide (fst (reveal ht))) `star`
-     ghost_pts_to tail.ghost half (hide (snd (reveal ht))) `star`
-     Q.queue (hide (fst (reveal ht))) (hide (snd (reveal ht)))))
+   (ghost_pts_to head.ghost half x `star`
+    ghost_pts_to tail.ghost half y `star`
+    Q.queue x y)
    (fun _ -> queue_invariant head tail)
- = rewrite_context()
+ = let w = Ghost.hide (Ghost.reveal x, Ghost.reveal y) in
+   change_slprop
+    (ghost_pts_to head.ghost half x `star`
+     ghost_pts_to tail.ghost half y `star`
+     Q.queue x y)
+    (ghost_pts_to head.ghost half (hide (fst (reveal w))) `star`
+     ghost_pts_to tail.ghost half (hide (snd (reveal w))) `star`
+     Q.queue (hide (fst (reveal w))) (hide (snd (reveal w))))
+    (fun _ -> ());
+   intro_exists w (fun w -> ghost_pts_to head.ghost half (hide (fst (reveal w))) `star`
+                         ghost_pts_to tail.ghost half (hide (snd (reveal w))) `star`
+                         Q.queue (hide (fst (reveal w))) (hide (snd (reveal w))))
 
 
 noeq
@@ -49,22 +61,32 @@ type t (a:Type0) = {
   inv : inv (queue_invariant head tail)
 }
 
+let new_qptr (#a:_) (q:Q.t a)
+  : SteelT (q_ptr a)
+           emp
+           (fun qp -> ghost_pts_to qp.ghost half q)
+  = let ptr = alloc q in
+    let ghost = ghost_alloc q in
+    ghost_share ghost;
+    intro_exists (Ghost.hide q)
+                 (fun q -> pts_to ptr full q `star` ghost_pts_to ghost half q);
+    let lock = Steel.SpinLock.new_lock (h_exists (fun q -> pts_to ptr full q `star` ghost_pts_to ghost half q)) in
+    let res = { ptr; ghost; lock} in
+    change_slprop (ghost_pts_to ghost half q)
+                  (ghost_pts_to res.ghost half q)
+                  (fun _ -> ());
+    res
+
 let new_queue (#a:_) (x:a)
   : SteelT (t a) emp (fun _ -> emp)
-  = sladmit()
-
-let intro_exists (#a:Type) (#opened_invariants:_)
-                 (x:Ghost.erased a)
-                 (p:a -> slprop)
-  : SteelAtomicT unit opened_invariants unobservable
-                 (p (Ghost.reveal x))
-                 (fun _ -> h_exists p)
-  = change_slprop (p (Ghost.reveal x))
-                  (h_exists p)
-                  (fun m -> Steel.Memory.intro_h_exists (Ghost.reveal x) p m)
+  = let hd = Q.new_queue x in
+    let head = new_qptr hd in
+    let tail = new_qptr hd in
+    pack_queue_invariant _ _ head tail;
+    let inv = new_invariant Set.empty (queue_invariant head tail) in
+    { head; tail; inv }
 
 #push-options "--ide_id_info_off"
-
 let enqueue_core (#a:_) (#u:_) (#x:Q.cell a{x.Q.next==null}) (hdl:t a) (tl:Q.t a) (node:Q.t a) (_:unit)
   : SteelAtomicT unit u observable
     (queue_invariant hdl.head hdl.tail `star`
@@ -99,7 +121,6 @@ let enqueue_core (#a:_) (#u:_) (#x:Q.cell a{x.Q.next==null}) (hdl:t a) (tl:Q.t a
     Steel.Effect.Atomic.intro_exists w (fun w -> (ghost_pts_to hdl.head.ghost half (hide (fst (reveal w))) `star`
                                                ghost_pts_to hdl.tail.ghost half (hide (snd (reveal w))) `star`
                                                Q.queue (hide (fst (reveal w))) (hide (snd (reveal w)))))
-
 
 
 let enqueue (#a:_) (hdl:t a) (x:a)
